---
layout: post
mathjax: true
title:  "This is my second post"
author: "Sandro Cavallari"
---

# Welcome

**Hello world**, this is my first Jekyll blog post.

$$ \frac{\delta E_{x}}{\delta t} = \frac{\delta f(z-ct)}{\delta t} = f^{\prime}(z - ct)\Big(\frac{\delta(z-ct)}{\delta t}\Big) = -c*f^{\prime}(z - ct) $$

$$
\label{eq:1}
\begin{align}
  & \phi(x,y) = \phi \left(\sum_{i=1}^n x_ie_i, \sum_{j=1}^n y_je_j \right)
  = \sum_{i=1}^n \sum_{j=1}^n x_i y_j \phi(e_i, e_j) = \\
  & (x_1, \ldots, x_n) \left( \begin{array}{ccc}
      \phi(e_1, e_1) & \cdots & \phi(e_1, e_n) \\
      \vdots & \ddots & \vdots \\
      \phi(e_n, e_1) & \cdots & \phi(e_n, e_n)
    \end{array} \right)
  \left( \begin{array}{c}
      y_1 \\
      \vdots \\
      y_n
    \end{array} \right)
\end{align}
$$


 $$k^, i^, j^* = \arg\max x^\top z_k^{(i:j)}$$.

I hope you like it $$\ref{eq:1}$$ !
